cedar-lean/Cedar/Thm/SymCC/Data.lean
@@ -14,7 +14,9 @@
  limitations under the License.
 -/
 
-import Cedar.Thm.SymCC.Data.Basic
-import Cedar.Thm.SymCC.Data.BitVec
-import Cedar.Thm.SymCC.Data.Hierarchy
-import Cedar.Thm.SymCC.Data.LT
+module
+
+public import Cedar.Thm.SymCC.Data.Basic
+public import Cedar.Thm.SymCC.Data.BitVec
+public import Cedar.Thm.SymCC.Data.Hierarchy
+public import Cedar.Thm.SymCC.Data.LT
